\\ \solution 
\begin{align}
    \vec{A}-\vec{F}&=\myvec{1\\-1}-\myvec{\frac{-3}{2}\\\frac{5}{2}}
    =\myvec{\frac{5}{2}\\\frac{-7}{2}}
    \\
    \vec{E}-\vec{D}&=\myvec{-1\\-3}-\myvec{\frac{-7}{2}\\\frac{1}{2}}
    =\myvec{\frac{5}{2}\\\frac{-7}{2}}
    \\
	\implies	\vec{A}-\vec{F} &= \vec{E}-\vec{D}
\end{align}
See \figref{fig:Triangle}, 
\begin{figure}
\centering
\includegraphics[width=\columnwidth]{solutions/1/2/7/figs/figure1.png}
\caption{$AFDE$ form a parallelogram in triangle ABC}
\label{fig:Triangle}
\end{figure}





















