\solution 
\begin{enumerate}
\item From 
	\eqref{eq:median-e}
	and
	\eqref{eq:median-g},
\begin{align}
		\label{eq:tri-pts/4} \vec{G}-\vec{B} &= \myvec{2 \\ -6},\, 
 \vec{E}-\vec{G} = \myvec{1 \\ -3} \\
	\implies \vec{G}-\vec{B} &= 2 \brak{ \vec{E}-\vec{G} }
	\\
	\text{or, }		\label{eq:tri-pts/8}\frac{BG}{GE} &=  2  
\end{align}		
\item Calculating the ratio of $GF$ and $CG$,
\begin{align}
		\label{eq:tri-pts/9} \vec{F}-\vec{G} &= \myvec{\frac{1}{2} \\ \frac{5}{2}} \\
		\label{eq:tri-pts/10} \vec{G}-\vec{C} &= \myvec{1 \\ 5} \\
		\label{eq:tri-pts/11} \norm{\vec{F}-\vec{G}} &= \sqrt{\brak{\frac{1}{2}}^{2} + \brak{\frac{5}{2}}^{2}} &= \frac{\sqrt{26}}{2} \\  
		\label{eq:tri-pts/12} \norm{\vec{G}-\vec{C}} &= \sqrt{1^2 + 5^2} &= \sqrt{26} \\
		\label{eq:tri-pts/13}\frac{CG}{GF} &= \frac{\norm{\vec{G}-\vec{C}}}{\norm{\vec{F}-\vec{G}}} &= \frac{\sqrt{26}}{\frac{\sqrt{26}}{2}} &= 2		
\end{align}
\item Calculating the ratio of $AG$ and $GD$,
\begin{align}
		\label{eq:tri-pts/14} \vec{G}-\vec{A} &= \myvec{-3 \\ 1} \\
		\label{eq:tri-pts/15} \vec{D}-\vec{G} &= \myvec{\frac{-3}{2} \\ \frac{1}{2}} \\
		\label{eq:tri-pts/16} \norm{\vec{G}-\vec{A}} &= \sqrt{\brak{-3}^{2}+1^2} &= \sqrt{10} \\
		\label{eq:tri-pts/17} \norm{\vec{D}-\vec{G}} &= \sqrt{\brak{\frac{-3}{2}}^{2}+\brak{\frac{1}{2}}^{2}} &= \frac{\sqrt{10}}{2} \\
		\label{eq:tri-pts/18}\frac{AG}{GD} &= \frac{\norm{\vec{G}-\vec{A}}}{\norm{\vec{D}-\vec{G}}} &= \frac{\sqrt{10}}{\frac{\sqrt{10}}{2}} &= 2 
\end{align}
\end{enumerate}
From \eqref{eq:tri-pts/8}, \eqref{eq:tri-pts/13}, \eqref{eq:tri-pts/18}
\begin{align}
		\frac{BG}{GE} = 
		\frac{CG}{GF} =
		\frac{AG}{GD} = 2
\end{align}
Hence verified.
